\documentclass{article}
\usepackage{graphicx}
\usepackage{amsmath}
\usepackage{array}
\usepackage[font=small, labelfont={sf,bf}, margin=1cm]{caption}
\usepackage{tabularx}
\usepackage{amssymb}



\date{Due:Sep 19 Edit: \today}
\title{PHYS 225 HW 3}
\author{James Liu}

\begin{document}
\maketitle
\begin{itemize}
    \item[1.]
    \begin{itemize}
        \item [a)]
        \[\begin{bmatrix}
            1&0&4\\0&1&2\\0&0&1
        \end{bmatrix}\times\begin{bmatrix}
            -1\\3\\1
        \end{bmatrix}=\begin{bmatrix}
            -1\cdot1+3\cdot0+1\cdot4\\
            -1\cdot0+3\cdot1+1\cdot2\\
            -1\cdot0+3\cdot0+1\cdot1
        \end{bmatrix}=\begin{bmatrix}
            3\\5\\1
        \end{bmatrix}\]
        
        \item [b)]
        \[\begin{bmatrix}
            1&0&a_1\\0&1&a_2\\0&0&1
        \end{bmatrix}\times\begin{bmatrix}
            b_1\\b_2\\1
        \end{bmatrix}=\begin{bmatrix}
            b_1\cdot1+b_2\cdot0+1\cdot a_1\\
            b_1\cdot0+b_2\cdot1+1\cdot a_2\\
            b_1\cdot0+b_2\cdot0+1\cdot1
        \end{bmatrix}=\begin{bmatrix}
            b_1+a_1\\b_2+a_2\\1
        \end{bmatrix}\]
        
        \item [c)]
        \[\begin{bmatrix}
            \text{cos}\theta&-\text{sin}\theta&x^0\\
            \text{sin}\theta&\text{cos}\theta&y^0\\
            0&0&1
        \end{bmatrix}\times \begin{bmatrix}
            x\\y\\1
        \end{bmatrix}= \begin{bmatrix}
            \text{cos}\theta \cdot x-\text{sin}\theta\cdot y+x^0\\
            \text{sin}\theta \cdot x+\text{cos}\theta\cdot y+y^0\\
            1
        \end{bmatrix}\]

        \item [d)] It is turing \(\overrightarrow{v}\) conter clockwise with degree of \(\theta\) and shifting its space's origin into \((x^0,y^0)\)
        \begin{figure}[h]
            \centering
            \includegraphics*[scale=0.10]{image/image1.jpeg}
        \end{figure}
    \end{itemize}
    \item[2.]
    \begin{itemize}
        \item [a)] \(M^i_i = 1-3+5 = 3\)
        \item [b)] \(\delta^i_i =n\)
        \item [c)] \(M^i_j\delta^j_i = \sum_{i}^{n}\sum_{j}^{n}M^i_j\delta^j_i = \{\sum_{i}^{n}\sum_{j}^{n}M^i_j|i=j\} = M^i_i\)
    \end{itemize}
\end{itemize}


\end{document}