\documentclass[a4paper,fleqn]{article}
\usepackage{graphicx}
\usepackage[fleqn]{amsmath}
\usepackage{array}
\usepackage[font=small, labelfont={sf,bf}, margin=1cm]{caption}
\usepackage{tabularx}
\usepackage{amssymb}


\title{\textbf{Homework \#2 }}
\author{James Liu}
\date{\ }


\begin{document}

\maketitle


\section*{Problem 1}
    
    \[
        \left |\frac{x}{x+1} \right |\leqslant 1 
    \]\[
        -1 \leqslant \frac{x}{x+1} \leqslant 1 
    \]
    1. suppose \(x+1 > 0\)
    \[
    -x-1 \leqslant x \leqslant x+1    
    \]\[
    -1 \leqslant 2x \leqslant 2x+1    
    \]\[
    - \frac {1} {2} \leqslant x\leqslant x+\frac1 2
    \]
    Because 
    \(\forall x \in \mathbb{R},\  x \leqslant x + \frac 1 2\)
    Therefore, solution set will be \(x\geqslant -\frac 1 2\) \\
    which is \(\left[-\frac 1 2, \infty\right)\)\\
    2. suppose \(x+1 < 0\)
    \[
    -x-1 \geqslant x \geqslant x+1    
    \]\[
    -1 \geqslant 2x \geqslant 2x+1    
    \]\[
    - \frac {1} {2} \geqslant x\geqslant x+\frac1 2
    \]
    Because
    \(\forall x \in \mathbb{R},\  x \leqslant x + \frac 1 2\). Therefore, there are no solution in this region.
    Therefore, the solution set is \(\left[-\frac 1 2, \infty\right)\).

\section*{Problem 2}
    \subsection*{a)}
        Because that \(f\) is increasing and \(g\) is decreasing, \(\forall x,y, \ x\in A, \text{and } y\in A \),
        if \(x<y, \ \text{then }f(x)\leqslant f(y)\). Similarly, if \( x<y, \ \text{then } g(x)\geqslant g(y)\), then \(-g(x)\leqslant -g(y)\).
        \(\forall x \in A, f-g \text{ at }x \ \text{equals to } f(x)-g(x)\), similarly, \(f-g \text{ at }y \ \text{equals to } f(y)-g(y)\).
        Recall previous inequalities of \(f(x)\leqslant f(y)\ \text{and } -g(x)\leqslant -g(y) \). Adding them will give
        \(f(x)-g(x) \leqslant f(y)-g(y)\) under that \(x<y\). Therefore, \(f-g\) is increasing.
    \subsection*{b)}
        If \(f\) is not increasing, then  \( \forall x,y \in A, \text{ when } x<y,\) there is \(f(x)>f(y)\). \\ 
        Therefore \(-1 \times f(x)< -1 \times f(y)\) which is \(-f(x)<-f(y)\) under \(x<y\). Therefore, \(-f\) is not decreasing.
\section*{Problem 3}
    \subsection*{a)}
    It is true.
        Because \(f,g\) are both odd, there is \(\forall x\in \mathbb{R}, \ f(-x)=-f(x)\) and \(g(-x)=-g(x)\). 
        Adding them will give \(f(-x)+g(-x)=-\left(f(x)+g(x)\right)\). Suppose \(h=f+g\), then the expression 
        turns \(h(-x)=-h(x)\) under \(\forall x \in \mathbb{R}\). Therefore, \(f+g\) is odd.
    \subsection*{b)}
    It is true.
        For \(f\) to be bounded, \(M\in \mathbb{R}, \ \text{ and} \ \exists M > 0\) so that \(\forall x \in \mathbb{R}, \ \left | f(x) \right | < M\)
        Similarly, for \(N\in \mathbb{R}\), and \(\exists N>0\) so that \(\forall x\in \mathbb{R}, \ |g(x)|<N\).
        Because \(M>0,\ N>0,\ |f(x)|\geqslant 0,\ |g(x)| \geqslant 0\), then multiply them together will give \(|f(x)|\cdot |g(x)|<N\cdot M\) Which is 
        equivalent to \(|f(x)\cdot g(x)|<N\cdot M\). Because \(N\) and \(M\) are all finite numbers, \(N\cdot M\) will also be finite number. Thus, \(f\cdot g\) is still bounded.
    \subsection*{c)}
    It is false.
        For example, if \(f(x)=e^x\) and \(g(x)=\frac x {e^x}\). \(f\cdot g = x\). \(\forall a \in \mathbb{R}, \ 
        -x = -x \). Thereofre, \(f\cdot g\) is an odd function. However, for example, take\(take x=1, \ and x=-1\). 
        \(f(1)=e^1\), and \(f(-1)=e^{-1}\). Because \(-e^1 \neq e^{-1}\), \(f(x)\) is not odd. Similarly, \(g(-1)=-e\)
        , and \(g(1)=\frac 1 e\). Because \(\frac 1 e \neq -e\), \(g(x)\) is also not odd.
    \subsection*{d)}
    It is false.
        For example, if \(f(x)=e^x\) and \(g(x) = \frac 1 {e^x}\), \(f(x)\cdot g(x) = 1\) which is bounded. While  \(e^x\) and \(\frac 1 {e^x}\) are all unbounded.
        Therefore, the statement is false.
\section*{Problem 4}
    1. If \(A=B\):\\ 
    Because \(A=B\), \(A \subseteq B, \text{ and }B\subseteq A\). Because \(A\subseteq B\), there is \(A\cup B = B\). Similarly, 
    because \(B\subseteq A\), \(A\cup B = A\). Thus,if \( A=B, A\cup B = A = B\). Because \(A\subseteq B\), there is \(A\cap B = A\). Similarly, 
    because \(B\subseteq A\), \(A\cap B = B\). Thus,if \( A=B, A\cap B = A = B\). Thus, if \( A=B, A\cup B = A\cap B\).
    \\2. If \(A\cap B = A\cup B\):\\
    Suppose \(x\in A\), then \(x\in A\cup B\). Because \(A\cap B = A\cup B\), \(x\in A\cap B\). Thus, \(x\in B\) which means 
    \(A \subseteq B\). Similarly , if \(y\in B\), then \(y\in A\cup B\), then \(y\in A\cap B\), and \(y\in B\) meaning \(B\subseteq A\). Thus, \(A=B\)
\section*{Problem 5}
    \subsection*{a)}
        Noting the compliment of a set \(A\) as \(A^X\). \(A-B\) gives a set that all element in \(A-B\) is in set \(A\)
        and not in set \(B\). Therefore \(B^X\) gives a set does not contain any element from set \(B\). 
        Thus, \(A-B\) can be noted as \(A\cap B^X\). \\
        Therefore,

        \begin{align*}
            A \triangle (B \triangle C) &=A\triangle ((B\cap C^X) \cup (C\cap B^X))             \\
                                        &=(A\cap((B\cap C^X) \cup (C\cap B^X))^X) \cup (A^X\cap((B\cap C^X) \cup (C\cap B^X)))\\
                                        &\text {using De Morgan's Law }\\
                                        &=(A\cap((B\cap C^X)^X \cap (C\cap B^X)^X)) \cup ((A^X\cap (B\cap C^X)) \cup (A^X\cap (C\cap B^X)))\\
                                        &=\mathbf{(A\cap (B^X\cup C)\cap (B \cup C^X))}\cup ((A^X \cap B\cap C^X)\cup (A^X\cap B^X \cap C))\\
                                        &=\mathbf{(((A\cap B)\cup (A\cap C^X)) \cap (B^X\cup C))}\cup ((A^X \cap B\cap C^X)\cup (A^X\cap B^X \cap C))\\
                                        &=((A\cap B)\cap (B^X\cup C)) \cup \mathbf{((A\cap C^X) \cap (B^X\cup C))}\cup ((A^X \cap B\cap C^X)\cup (A^X\cap B^X \cap C))\\
                                        &=((A\cap B)\cap (B^X\cup C)) \cup ((A\cap C^X \cap B^X)\cup \\ & \ \ \ \ \ \mathbf{(A\cap C^X \cap C)})\cup ((A^X \cap B\cap C^X)\cup (A^X\cap B^X \cap C))\\
                                        &=\mathbf{((A\cap B)\cap (B^X\cup C))} \cup ((A\cap C^X \cap B^X)\cup \mathbf{\varnothing})\cup ((A^X \cap B\cap C^X)\cup (A^X\cap B^X \cap C))\\
                                        &=((A\cap B \cap B^X)\cup (A \cap B \cap C))\cup\\ & \ \ \ \ \  ((A\cap C^X \cap B^X))\cup ((A^X \cap B\cap C^X)\cup (A^X\cap B^X \cap C))\\
                                        &=(A \cap B \cap C)\cup ((A\cap C^X \cap B^X))\cup ((A^X \cap B\cap C^X)\cup (A^X\cap B^X \cap C))\\
            (A \triangle B) \triangle C &=C\triangle ((B\cap A^X) \cup (A\cap B^X))             \\
                                        &=(C\cap((B\cap A^X) \cup (A\cap B^X))^X) \cup (C^X\cap((B\cap A^X) \cup (A\cap B^X)))\\
                                        &\text {using Ce Morgan's Law }\\
                                        &=(C\cap((B\cap A^X)^X \cap (A\cap B^X)^X)) \cup ((C^X\cap (B\cap A^X)) \cup (C^X\cap (A\cap B^X)))\\
                                        &=\mathbf{(C\cap (B^X\cup A)\cap (B \cup A^X))}\cup ((C^X \cap B\cap A^X)\cup (C^X\cap B^X \cap A))\\
                                        &=\mathbf{(((C\cap B)\cup (C\cap A^X)) \cap (B^X\cup A))}\cup ((C^X \cap B\cap A^X)\cup (C^X\cap B^X \cap A))\\
                                        &=((C\cap B)\cap (B^X\cup A)) \cup \mathbf{((C\cap A^X) \cap (B^X\cup A))}\cup ((C^X \cap B\cap A^X)\cup (C^X\cap B^X \cap A))\\
                                        &=((C\cap B)\cap (B^X\cup A)) \cup ((C\cap A^X \cap B^X)\cup \\ & \ \ \ \ \ \mathbf{(C\cap A^X \cap A)})\cup ((C^X \cap B\cap A^X)\cup (C^X\cap B^X \cap A))\\
                                        &=\mathbf{((C\cap B)\cap (B^X\cup A))} \cup ((C\cap A^X \cap B^X)\cup \mathbf{\varnothing})\cup ((C^X \cap B\cap A^X)\cup (C^X\cap B^X \cap A))\\
                                        &=((C\cap B \cap B^X)\cup (C \cap B \cap A))\cup\\ & \ \ \ \ \  ((C\cap A^X \cap B^X))\cup ((C^X \cap B\cap A^X)\cup (C^X\cap B^X \cap A))\\
                                        &=(C \cap B \cap A)\cup ((C\cap A^X \cap B^X))\cup ((C^X \cap B\cap A^X)\cup (C^X\cap B^X \cap A))\\
        \end{align*}
        Therefore, \(A \triangle (B \triangle C)=(A \triangle B) \triangle C\)
    \subsection*{b)}
        The statement proofing will here be: \(A\triangle B \triangle C\) 
        can be characterize as the set of element belonging exactlly one or all of three of the sets A,B,C, which is the shaded area of figure 1.
        \begin{figure}[h]
            \centering
            \includegraphics*[scale = 0.5]{image/Venn.png}
            \caption{}
        \end{figure}
        
        from the previous answer, the solution set of \(A\triangle B \triangle C\) is:\\
        \[(A \cap B \cap C)\cup ((A\cap C^X \cap B^X))\cup ((A^X \cap B\cap C^X)\cup (A^X\cap B^X \cap C))\]
            1. \((A \cap B \cap C)\)\\
                Suppose \(x\in (A \cap B \cap C)\), then \(x\in A, \ x\in B, \ x \in C\)\\
            2. \((A\cap C^X \cap B^X)\)\\
                Suppose \(x\in (A\cap C^X \cap B^X)\), it means that \(x\in A\), and \(x\notin B\), and \(x\notin C\).
            Similarly, for \((C^X \cap B\cap A^X)\) and \((C^X\cap B^X \cap A)\), they means that \(x\in B, \ x\notin A, \ x \notin C\), \
            and \(x\in C, \ x\notin A, \ x \notin B\)
        Therefore, \(A\triangle B \triangle C\) 
        can be characterize as the set of element belonging exactlly one or all of three of the sets A,B,C.

\end{document}

Suppose \(x\in A\cap B\), then \(x \notin A-B\) and \(x\notin B-A\). Therefore, \(x\notin A \triangle B\). Because there is no
extra element introduced in \(A \triangle B\), \(A\triangle B \in A+B\)