\documentclass{article}
\usepackage{graphicx}
\usepackage{amsmath}
\usepackage{array}
\usepackage[font=small, labelfont={sf,bf}, margin=1cm]{caption}
\usepackage{tabularx}
\usepackage{amssymb}



\date{Due:Nov 22 Edit: \today}
\title{NPRE200 HW 5}
\author{James Liu}

\begin{document}
\maketitle
\begin{itemize}
    \item [1.]
    \begin{itemize}
        \item [a)]
        \begin{align*}
            \frac{\text{d}n}{\text{d}t}&=S+P-A+R\\
            &=S+(\nu-1)\Sigma_f\phi-\Sigma_c\phi+D\nabla^2\phi
        \end{align*}
        \item [b)]
        \begin{align*}
            \frac{\text{d}n}{\text{d}t}&=S+P-A+R\\
            &=S+(\eta-1)\Sigma_a\phi+D\nabla^2\phi
        \end{align*}
        \item [c)]
        \begin{align*}
            \frac{\text{d}n}{\text{d}t}&=S+P-A+R=0\\
            0&=S+(\eta-1)\Sigma_a\phi+D\nabla^2\phi
        \end{align*}
        \item [d)]
        \begin{align*}
            \frac{\text{d}n}{\text{d}t}&=S+P-A+R=0\\
            0&=S-\Sigma_a\phi+D\nabla^2\phi
        \end{align*}
    \end{itemize}
    \item [2.]
    \begin{itemize}
        \item [a)]
        \begin{align*}
            \frac{\text{d}n}{\text{d}t}&=S-\Sigma_a\phi+D\nabla^2\phi=0\\
            0&=S-\Sigma_a\phi+D\nabla^2\phi\\
            -D\nabla^2\phi&=S-\Sigma_a\phi\\
            -\nabla^2\phi+\frac{\Sigma_a}{D}\phi&=\frac{S}{D}\\
            -\nabla^2\phi+\frac{1}{L^2}\phi&=\frac{S}{D}
        \end{align*}
        \item [b)]
        \begin{align*}
            \nabla^2\phi-\frac{1}{L^2}\phi&=0\\
            \nabla^2=\frac{\text{d}^2}{\text{d}x^2}\\
            \frac{\text{d}^2\phi}{\text{d}x^2}-\frac{1}{L^2}\phi&=0\\
            \phi&=Ae^{xp}+Ce^{-xp}\\
            \phi(x)&=Ae^{\frac{x}{L}}+Ce^{-\frac{x}{L}}\\
            \phi(0)&=\phi_0\\
            \phi(\infty)&=0\\
            0&=Ae^{xp}+Ce^{-xp}\\
            0&=A\cdot\infty+C\cdot 0\\
            A&=0\\
            \phi_0&=Ae^{xp}+Ce^{-xp}\\
            \phi_0&=C\cdot 1\\
            C&=\phi_0\\
            \phi(x)&=\phi_0e^{-\frac{x}{L}}
        \end{align*}
    \end{itemize}
    \item [3.]
    \begin{align*}
        \frac{\text{d}^2\phi}{\text{d}x^2}-\frac{1}{L^2}\phi&=-\frac{S}{D}\\
        \phi_g(x)=Ae^{\frac{x}{L}}+Ce^{-\frac{x}{L}}\\
        \text{Take a particular solution }\phi_{pi}\\
        \frac{\text{d}^2\phi}{\text{d}x^2}p^2\phi&=Q\\
        \phi_{pi}&=\frac{Q}{p^2}\\
        &=\frac{S/D}{1/L^2}\\
        &=\frac{L^2}{D}\cdot S \\
        &= \frac{1}{D/L^2}\cdot S\\
        &= \frac{S}{\Sigma_a}
        \phi(x)=Ae^{\frac{x}{L}}+Ce^{-\frac{x}{L}}+\frac{S}{\Sigma_a}
    \end{align*}
    \newpage
    \item [4.]
    \begin{itemize}
        \item [a)]
        \begin{align*}
            \phi&=\phi_0e^{-\frac{x}{L}}\\
            J_x(x)&=J^+_x(x)-J^-_x(x)\\
            J^{\pm }_x(x)&=\frac{1}{4}\phi(x)\mp \frac{1}{2}D\frac{\text{d}}{\text{d}x}\phi(x)\\
            J^{\pm }_x(0)&=\frac{1}{4}\phi(0)\mp \frac{1}{2}D\frac{\text{d}}{\text{d}x}\phi(x)\\
            &=\frac{1}{4}\phi_0\mp\frac{1}{2}D\left.\left[\frac{\text{d}}{\text{d}x}\phi_0e^{-\frac{x}{L}}\right]\right|_{x=0}\\
            &=\frac{1}{4}\phi_0\pm\frac{1}{2}\frac{D}{L}\phi_0\\
            \phi_0&=J^+_x(0)\left(\frac{1}{4}+\frac{D}{2L}\right)^{-1}\\
            \phi&=\phi_0e^{-\frac{x}{L}}\\
            \phi&=J^+_x(0)\left(\frac{1}{4}+\frac{D}{2L}\right)^{-1}e^{-\frac{x}{L}}
        \end{align*}
        \item [b)]
        \begin{align*}
            \alpha &=\frac{J_x^-(0)}{J^+_x(0)}\\
            &=\frac{\frac{1}{4}+\frac{D}{2L}}{\frac{1}{4}-\frac{D}{2L}}\\
            &=\frac{L-2D}{L+2D}
        \end{align*}
    \end{itemize}
\end{itemize}
\end{document}



