\documentclass{article}
\usepackage{graphicx}
\usepackage{amsmath}
\usepackage{array}
\usepackage[font=small, labelfont={sf,bf}, margin=1cm]{caption}
\usepackage{tabularx}
\usepackage{amssymb}



\date{Due: Nov 1 Edit: \today}
\title{MATH 461 Homework 8}
\author{James Liu}

\begin{document}
\maketitle
\begin{itemize}
    \item [6.27]
    \begin{itemize}
        \item [a)]    \begin{align*}
            f_Z(z)&=\int_{0}^{\infty} f_{Z,W}(z,w)dw\\
            &=\int_{0}^{\infty}\lambda_1\lambda_2e^{-\lambda_1zw}e^{-\lambda_2w}\frac{1}{w}dw\\
            &=\lambda_1\lambda_2\int_{0}^{\infty}\frac{1}{w}e^{-(\lambda_1z+\lambda_2)w}dw\\
            &=\frac{\lambda_1\lambda_2}{\lambda_1z+\lambda_2};z\geq0
        \end{align*}
        \item [b)]
        \begin{align*}
            P(X_1<X_2)&=\int_{0}^{\infty}P(X_1<x)\times f_{X_2}(x)dx\\
            &=\int_{0}^{\infty}(1-e^{-\lambda_1x})\lambda_2e^{-\lambda_2x}dx\\
            &=\lambda_2\int_{0}^{\infty}e^{-\lambda_2x}dx - \lambda_2\int_{0}^{\infty}e^{-(\lambda_1+\lambda_2)x}dx\\
            &=\lambda_2\frac{1}{\lambda_2}-\lambda_2\frac{1}{\lambda_1+\lambda_2}\\
            &=\frac{\lambda_1}{\lambda_1+\lambda_2}
        \end{align*}
    \end{itemize}
    \item [6.29]
    \begin{itemize}
        \item [a)] \(\mu = 2200\times 2 = 4400\) and \(\sigma = 230 \times \sqrt{2}=325.27\).\(z = (5000-4400)/325.27=1.84\)
        \(P(x>5000)=P(z>1.845)=1-P(z<1.845)=1-0.9671=0.0329\)
        \item [b)] \(z = (2000-2200)/230 = -\frac{200}{230} = -0.87\)
        \(P(X>2000)=1-P(z<-0.87)=1-0.1922=0.8078\)
        \begin{align*}
            P(X\geq 2)&=P(X=2)+P(X=3)\\
            &=\binom{3}{2}(0.8078)^2(1-0.8078)+\binom{1}{1}(0.8078)^3\\
            &=0.9034
        \end{align*}
    \end{itemize}
    \item [6.31]
    \begin{itemize}
        \item [a)] \(\mu_x=n_1p_1=50.4\) \(\sigma_X^2 = n_1p_1(1-p_1)=37.6992\).\\
                    \(\mu_y=n_2p_2=47.2\) \(\sigma_Y^2 = n_2p_2(1-p_2)=36.0608\).\\
                    \(\mu_z=\mu_X+\mu_y = 97.6\) \(\sigma_Z^2 = \sigma_X^2+\sigma_Y^2=73.76\)\\
                    \(\sigma_Z = 8.5884\)\\
                    \begin{align*}
                        P(Z\geq 110)&=1-P(z<\frac{110-0.5-97.6}{8.5884})\\
                        &=1-0.9177\\
                        &=0.0823 
                    \end{align*}
        \item [b)] \(E(Y-X)=E(Y)-E(X)=-3.2\)
        \begin{align*}
            P(D\geq 0)&=P(z\geq \frac{0-3.2-0.5}{8.85884})\\
            &=0.3783
        \end{align*}

    \end{itemize}
    \item [6.34]
    \begin{itemize}
        \item [a)] 
        \begin{align*}
            P(N>2)&=1-P(N=0,1,2)\\
            &=1-e^{-2.2}-2.2e^{-2.2}-\frac{2.2^2}{2!}e^{-2.2}\\
            &=0.3773
        \end{align*}
        \item [b)]
        \begin{align*}
            P(N_1>4)&=1-\sum_{k=0}^4 \frac{4.4^k}{k!}e^{-4.4}\\
            &=0.44882
        \end{align*}
        \item [c)]
        \begin{align*}
            P(N_2>5)&=1-P(N_2=0,1,2,3,4,5)\\
            &=1-\sum_{k=0}^4 \frac{6.6^k}{k!}e^{-6.6}\\
            &=0.64533
        \end{align*}
    \end{itemize}
    \item [6.38]
    \begin{itemize}
        \item [a)]
        \begin{align*}
            P(Y=y,X=x)&=P(Y=y|X=x)\times P(X=x)\\
            &=\frac{1}{x}\times \frac{1}{5}\\
            &=\frac{1}{5x}
        \end{align*}
        \item [b)]
        \begin{align*}
            P(Y=i)&=\sum_{x=i}^{5}P(Y=i,X=x)\\
            &=\sum_{x=i}^5(\frac{1}{5x})
            P(X|Y=i)&=\frac{\frac{1}{5x}}{\sum_{x=i}^5(\frac{1}{5x})}
        \end{align*}
        \item [c)]No they are not as \(P(Y=y)\times P(X=x)\neq P(Y=y,X=x)\)
    \end{itemize}
    \item [6.40]
    \begin{itemize}
        \item [a)]
        \begin{tabular}{c|c|c}
            x&1&2\\ \hline
            \(P(x|y=1)\)&1/2&1/2\\ \hline 
            \(P(x|y=2)\)&1/3&2/3\\
        \end{tabular}
        \item [b)] They are not independent.
        \begin{align*}
            p_{x,y}(1,1)=1/8\\
            p_x(1)=3/8\\
            p_y(1)=1/4\\
            p_y(1)p_x(1)=3/32\neq p_{x,y}(1)
        \end{align*}
        \item [c)]
        \begin{itemize}
            \item [i.]
            \begin{align*}
                P(XY\leq3)&=P(1,1)+P(1,2)+P(2,1)\\
                &=1/8+1/4+1/8\\
                &=1/2
            \end{align*}
            \item [ii.]
            \begin{align*}
                P(X+Y>2)&=1-P(1,1)\\
                &=7/8
            \end{align*}
            \item [iii.]
            \begin{align*}
                P(X/y>1)&=P(2,1)\\
                &=1/8
            \end{align*}
        \end{itemize}
    \end{itemize}
    \item [6.41]
    \begin{itemize}
        \item [a)]
        \begin{align*}
            f(x)&=\int_{0}^{\infty}xe^{-x(y+1)}dy\\
            &=e^{-x}\\
            f(y)&=\int_{0}^{\infty}xe^{-x(y+1)}dx = \frac{1}{(y+1)^2}\\
            Y=y,f(x,y)=\frac{f(x,y)}{f(y)}&=\frac{xe^{-x(y+1)}}{\frac{1}{(y+1)^2}}\\
            &=x(y+1)^2e^{-x(y+1)}\\
            X=x,f(x,y)=\frac{f(x,y)}{f(x)}&=\frac{xe^{-x(y+1)}}{e^{-x}}\\
            &=xe^{-xy}
        \end{align*}
        \item [b)]
        \begin{align*}
            P(XY<z)&=\int_{0}^{\infty}\int_{0}^{z/x} f(x,y)dydx\\
            &=\int_{0}^{\infty}\int_{0}^{z/x} xe^{-x(1+y)}dydx\\
            &=\int_{0}^{\infty}(1-e^{-z}x^{-x})dx\\
            &=(1+e^{-x})
        \end{align*}
    \end{itemize}
    \item [6.42]\
    \begin{itemize}
        \item [\(t\leq x\)] \[P(Y\leq t|X=x)=\frac{3}{2x^3}(x^2(t+x)-t^3/3+x^3/3)\]
        \item [\(t<-x\)] \[P(Y\leq t|X=x)=0\]
        \item [\(t>x\)] \[P(Y\leq t|X=x)=1\]
    \end{itemize}
\end{itemize}

\end{document}